WIP: working commit

coq/v2/Examples/Negator.v
@@ -7,12 +7,14 @@ Require Import Trustformer.v2.Syntax.
 Require Import Trustformer.v2.Semantics.
 Require Import Trustformer.v2.Synthesis.
 
+Require Import Coq.Logic.EqdepFacts.
+
 Require Import Hammer.Plugin.Hammer.
 Set Hammer GSMode 63.
 
 (*
     An example specification and synthesis of a simple negator module.
-    The hardware module has a single internal state register (32 bits) and supports two actions (nop, neg).
+    The hardware module has a single internal state register (32 bits) and supports four actions (nop, neg, read, write).
     Actions are triggered through a command register, where the first 1 bit indicates if the command is valid,
     and the remaining bits indicate the action to perform.
 
@@ -27,6 +29,8 @@ Section FunctionalSpecification.
     Inductive fs_action :=
     | fs_act_nop
     | fs_act_neg
+    | fs_act_read
+    | fs_act_write
     .
 
     Inductive fs_states :=
@@ -34,9 +38,11 @@ Section FunctionalSpecification.
     .
 
     Inductive fs_inputs :=
+    | fs_in_val
     .
 
     Inductive fs_outputs :=
+    | fs_out_val
     .
 
     Definition fs_states_size (x: fs_states) : nat :=
@@ -46,10 +52,12 @@ Section FunctionalSpecification.
 
     Definition fs_inputs_size (x: fs_inputs) : nat := 
     match x with
+    | fs_in_val => sz
     end.
 
     Definition fs_outputs_size (x: fs_outputs) : nat := 
     match x with
+    | fs_out_val => sz
     end.
 
     Definition fs_states_t := tf_states_type fs_states fs_states_size. 
@@ -67,11 +75,16 @@ Section FunctionalSpecification.
         match act with
         | fs_act_nop => tf_nop _ _ _ 
         | fs_act_neg => tf_neg _ _ _ fs_st_val
+        | fs_act_read => tf_output _ _ _ fs_st_val fs_out_val
+        | fs_act_write => tf_input _ _ _ fs_st_val fs_in_val
         end.
 
     Definition fs_step := tf_op_step_commit fs_states _ fs_inputs fs_outputs fs_states_size fs_inputs_size.
+    Definition fs_output := tf_op_outputs fs_states _ fs_inputs fs_outputs _ fs_states_size fs_inputs_size fs_outputs_size.
     
     Section Examples.
+        Definition bits_10 := Bits.of_nat sz 10.
+        Definition bits_neg10 := Bits.neg (Bits.of_nat sz 10).
 
         Definition s_init := ContextEnv.(create) fs_states_init.
         Example s_example : ContextEnv.(getenv) s_init fs_st_val = bits_false.
@@ -79,14 +92,42 @@ Section FunctionalSpecification.
 
         Definition s1_trans := fs_transitions fs_act_nop.
         Definition s1_state := fs_step s_init (fun _ => Bits.zero) s1_trans.
-        Example s1_example : ContextEnv.(getenv) s1_state fs_st_val = bits_false.
+        Definition s1_output := fs_output s_init (fun _ => Bits.zero) (ContextEnv.(create) (fun _ => Bits.zero)) s1_trans.
+        Example s1_example_state : ContextEnv.(getenv) s1_state fs_st_val = bits_false.
         Proof. ssimpl. Qed.
-        
-        Definition s2_trans := fs_transitions fs_act_neg.
-        Definition s2_state := fs_step s_init (fun _ => Bits.zero) s2_trans.
-        Example s2_example : ContextEnv.(getenv) s2_state fs_st_val = bits_true.
+        Example s1_example_output : ContextEnv.(getenv) s1_output fs_out_val = bits_false.
+        Proof. ssimpl. Qed.
+
+        Definition s2_trans := fs_transitions fs_act_write.
+        Definition s2_state := fs_step s_init (fun x => match x with fs_in_val => bits_10 end) s2_trans.
+        Definition s2_output := fs_output s_init (fun x => match x with fs_in_val => bits_10 end) (ContextEnv.(create) (fun _ => Bits.zero)) s2_trans.
+        Example s2_example : ContextEnv.(getenv) s2_state fs_st_val = bits_10.
         Proof. 
             cbn -[vect_to_list]. sauto.
+        Qed.
+        Example s2_example_output : ContextEnv.(getenv) s2_output fs_out_val = bits_false.
+        Proof. ssimpl. Qed.
+        
+        Definition s3_trans := fs_transitions fs_act_neg.
+        Definition s3_state := fs_step s2_state (fun _ => Bits.zero) s3_trans.
+        Definition s3_output := fs_output s2_state (fun _ => Bits.zero) (ContextEnv.(create) (fun _ => Bits.zero)) s3_trans.
+        Example s3_example : ContextEnv.(getenv) s3_state fs_st_val = bits_neg10.
+        Proof. 
+            cbn -[vect_to_list Bits.neg]. sauto.
+        Qed.
+        Example s3_example_output : ContextEnv.(getenv) s3_output fs_out_val = bits_false.
+        Proof. ssimpl. Qed.
+
+        Definition s4_trans := fs_transitions fs_act_read.
+        Definition s4_state := fs_step s3_state (fun _ => Bits.zero) s4_trans.
+        Definition s4_output := fs_output s3_state (fun _ => Bits.zero) (ContextEnv.(create) (fun _ => Bits.zero)) s4_trans.
+        Example s4_example : ContextEnv.(getenv) s4_state fs_st_val = bits_neg10.
+        Proof. 
+            cbn -[vect_to_list]. sauto.
+        Qed.
+        Example s4_example_output : ContextEnv.(getenv) s4_output fs_out_val = bits_neg10.
+        Proof.
+            cbn -[vect_to_list Bits.neg]. sauto.
         Qed.
 
     End Examples.
@@ -140,7 +181,7 @@ Section Synthesis.
                         koika_rule_names := Synthesis.rule_names tf_ctx;
                         koika_rule_external := (fun _ => false);
                         koika_scheduler := system_schedule;
-                        koika_module_name := "V2Example_InternalNegator" |};
+                        koika_module_name := "V2Example_Negator" |};
 
       ip_sim := {| sp_ext_fn_specs fn := {| efs_name := show fn; efs_method := false |};
                   sp_prelude := None |};
@@ -154,5 +195,5 @@ End Synthesis.
 
 Definition prog := Interop.Backends.register package.
 Set Extraction Output Directory "build".
-Extraction "V2Example_InternalNegator.ml" prog.
+Extraction "V2Example_Negator.ml" prog.
 
