coq/v2/Syntax.v
@@ -8,13 +8,17 @@ Set Hammer GSMode 63.
 
 Section TrustformerSyntax.
 
-    (* Given some variables we define our syntax *)
+    (* Given some variables, inputs and outputs we define our syntax *)
     Context (states_var: Type).
+    Context (inputs_var: Type).
+    Context (outputs_var: Type).
 
     (* Atomic operations on variables *)
     Inductive tf_ops :=
         | tf_nop (* No operation *)
         | tf_neg (x : states_var) (* Negate a variable *)
+        | tf_input (x : states_var) (y : inputs_var) (* Read input into variable *)
+        | tf_output (x : states_var) (y : outputs_var) (* Write variable to output *)
         . 
 
 End TrustformerSyntax.
